NuInstructions.thy
@@ -13,6 +13,7 @@ theory NuInstructions
 begin
 
 declare Nat.One_nat_def[simp del] Num.add_2_eq_Suc'[simp del] split_paired_All[simp del]
+declare Separation_assoc[simp]
 
 text \<open>Basic instructions\<close>
 
@@ -31,7 +32,7 @@ subsubsection \<open>drop\<close>
 definition op_drop :: "('a::lrep) \<times> ('r::stack) \<longmapsto> 'r" where
   "op_drop x = (case x of (h,a,r) \<Rightarrow> Success (h,r))"
 declare op_drop_def[\<nu>instr]
-theorem drop_\<nu>app: "\<^bold>p\<^bold>r\<^bold>o\<^bold>c op_drop \<blangle> R\<heavy_comma> X\<heavy_comma> \<^bold>h\<^bold>e\<^bold>a\<^bold>p H \<longmapsto> R\<heavy_comma> \<^bold>h\<^bold>e\<^bold>a\<^bold>p H \<brangle>"
+theorem drop_\<nu>app: "\<^bold>p\<^bold>r\<^bold>o\<^bold>c op_drop \<blangle> R\<heavy_comma> X\<heavy_comma> \<^bold>h\<^bold>e\<^bold>a\<^bold>p Nothing \<longmapsto> R\<heavy_comma> \<^bold>h\<^bold>e\<^bold>a\<^bold>p Nothing \<brangle>"
   unfolding \<nu>def op_drop_def by (auto simp add: nu_exps)
 
 subsubsection \<open>duplication\<close>
@@ -39,7 +40,7 @@ subsubsection \<open>duplication\<close>
 definition op_dup :: "('a::lrep) \<times> ('r::stack) \<longmapsto> ('a \<times> 'a \<times> 'r)"
   where "op_dup x = (case x of (h,a,r) \<Rightarrow> Success (h, a, a, r))"
 declare op_dup_def[\<nu>instr]
-theorem dup_\<nu>app: "\<^bold>p\<^bold>r\<^bold>o\<^bold>c op_dup \<blangle> R\<heavy_comma> X\<heavy_comma> \<^bold>h\<^bold>e\<^bold>a\<^bold>p H \<longmapsto> R\<heavy_comma> X\<heavy_comma> X\<heavy_comma> \<^bold>h\<^bold>e\<^bold>a\<^bold>p H\<brangle>"
+theorem dup_\<nu>app: "\<^bold>p\<^bold>r\<^bold>o\<^bold>c op_dup \<blangle> R\<heavy_comma> X\<heavy_comma> \<^bold>h\<^bold>e\<^bold>a\<^bold>p Nothing \<longmapsto> R\<heavy_comma> X\<heavy_comma> X\<heavy_comma> \<^bold>h\<^bold>e\<^bold>a\<^bold>p Nothing\<brangle>"
   unfolding \<nu>def op_dup_def by (auto simp add: nu_exps)
 
 
@@ -51,9 +52,9 @@ definition op_depair :: "(('b::lrep) \<times> ('a::lrep)) \<times> ('r::stack) \
   where "op_depair = (\<lambda>(h,(b,a),r). Success (h,a,b,r))"
 (* declare op_pair_def[\<nu>instr] op_depair_def[\<nu>instr] *)
 
-lemma pr_\<nu>app: "\<^bold>p\<^bold>r\<^bold>o\<^bold>c op_pair \<blangle> R \<heavy_comma> a \<tycolon> A \<heavy_comma> b \<tycolon> B\<heavy_comma> \<^bold>h\<^bold>e\<^bold>a\<^bold>p H \<longmapsto> R \<heavy_comma> (a,b) \<tycolon> (A \<cross_product> B)\<heavy_comma> \<^bold>h\<^bold>e\<^bold>a\<^bold>p H \<brangle>"
+lemma pr_\<nu>app: "\<^bold>p\<^bold>r\<^bold>o\<^bold>c op_pair \<blangle> R \<heavy_comma> a \<tycolon> A \<heavy_comma> b \<tycolon> B\<heavy_comma> \<^bold>h\<^bold>e\<^bold>a\<^bold>p Nothing \<longmapsto> R \<heavy_comma> (a,b) \<tycolon> (A \<cross_product> B)\<heavy_comma> \<^bold>h\<^bold>e\<^bold>a\<^bold>p Nothing \<brangle>"
   unfolding \<nu>def  op_pair_def by (auto simp add: nu_exps)
-lemma dpr_\<nu>app: "\<^bold>p\<^bold>r\<^bold>o\<^bold>c op_depair \<blangle> R \<heavy_comma> (a,b) \<tycolon> (A \<cross_product> B)\<heavy_comma> \<^bold>h\<^bold>e\<^bold>a\<^bold>p H \<longmapsto> R \<heavy_comma> a \<tycolon> A \<heavy_comma> b \<tycolon> B\<heavy_comma> \<^bold>h\<^bold>e\<^bold>a\<^bold>p H \<brangle>"
+lemma dpr_\<nu>app: "\<^bold>p\<^bold>r\<^bold>o\<^bold>c op_depair \<blangle> R \<heavy_comma> (a,b) \<tycolon> (A \<cross_product> B)\<heavy_comma> \<^bold>h\<^bold>e\<^bold>a\<^bold>p Nothing \<longmapsto> R \<heavy_comma> a \<tycolon> A \<heavy_comma> b \<tycolon> B\<heavy_comma> \<^bold>h\<^bold>e\<^bold>a\<^bold>p Nothing \<brangle>"
   unfolding \<nu>def  op_depair_def by (auto simp add: nu_exps)
 
 lemma hpr_\<nu>app: "\<^bold>c\<^bold>a\<^bold>s\<^bold>t H \<heavy_asterisk> h1 \<tycolon> H1 \<heavy_asterisk> h2 \<tycolon> H2 \<longmapsto> H \<heavy_asterisk> (h2,h1) \<tycolon> H2 \<^emph> H1"
@@ -76,12 +77,12 @@ lemma op_let: " (\<And>p. p \<nuLinkL> A \<nuLinkR> a \<Longrightarrow> \<^bold>
 
 definition op_local_value :: " 'v::lrep \<Rightarrow> 's::stack \<longmapsto> 'v \<times> 's "
   where "op_local_value v = (\<lambda>(h,s). Success (h,v,s))"
-lemma op_local_value: "v \<nuLinkL> A \<nuLinkR> a \<Longrightarrow> \<^bold>p\<^bold>r\<^bold>o\<^bold>c op_local_value v \<blangle> S\<heavy_comma> \<^bold>h\<^bold>e\<^bold>a\<^bold>p H \<longmapsto> S\<heavy_comma> a \<tycolon> A\<heavy_comma> \<^bold>h\<^bold>e\<^bold>a\<^bold>p H \<brangle>"
+lemma op_local_value: "v \<nuLinkL> A \<nuLinkR> a \<Longrightarrow> \<^bold>p\<^bold>r\<^bold>o\<^bold>c op_local_value v \<blangle> S\<heavy_comma> \<^bold>h\<^bold>e\<^bold>a\<^bold>p Nothing \<longmapsto> S\<heavy_comma> a \<tycolon> A\<heavy_comma> \<^bold>h\<^bold>e\<^bold>a\<^bold>p Nothing \<brangle>"
   unfolding Procedure_def op_local_value_def by (auto simp add: nu_exps)
 
 ML_file "library/local_value.ML"
 
-\<nu>processor let_local_value 500 \<open>\<^bold>c\<^bold>u\<^bold>r\<^bold>r\<^bold>e\<^bold>n\<^bold>t blk \<^bold>r\<^bold>e\<^bold>s\<^bold>u\<^bold>l\<^bold>t\<^bold>s \<^bold>i\<^bold>n (R\<heavy_comma> x \<tycolon> X\<heavy_comma> \<^bold>h\<^bold>e\<^bold>a\<^bold>p H)\<close> \<open>let open Parse in
+\<nu>processor let_local_value 500 \<open>\<^bold>c\<^bold>u\<^bold>r\<^bold>r\<^bold>e\<^bold>n\<^bold>t blk [\<HH>] \<^bold>r\<^bold>e\<^bold>s\<^bold>u\<^bold>l\<^bold>t\<^bold>s \<^bold>i\<^bold>n (R\<heavy_comma> x \<tycolon> X\<heavy_comma> \<^bold>h\<^bold>e\<^bold>a\<^bold>p H)\<close> \<open>let open Parse in
   fn ctx => fn sequent => (($$$ "\<rightarrow>" || $$$ "--") -- list1 binding) >> (fn (keyword,idts) => fn _ =>
     Local_Value.mk_let (keyword = "--") (rev idts) sequent ctx
 ) end\<close>
@@ -112,7 +113,7 @@ subsubsection \<open>sel\<close>
 definition op_sel :: " (1 word \<times> 'a \<times> 'a \<times> 'r) \<longmapsto> ('a \<times> 'r)"
   where "op_sel s = (case s of (heap,c,b,a,r) \<Rightarrow> if c = 1 then Success (heap,a,r) else Success (heap,b,r))"
 
-lemma sel_\<nu>app: " \<^bold>p\<^bold>r\<^bold>o\<^bold>c op_sel \<blangle> R\<heavy_comma> a \<tycolon> T\<heavy_comma> b \<tycolon> T\<heavy_comma> c \<tycolon> \<bool>\<heavy_comma> \<^bold>h\<^bold>e\<^bold>a\<^bold>p H \<longmapsto> R\<heavy_comma> (if c then a else b) \<tycolon> T\<heavy_comma> \<^bold>h\<^bold>e\<^bold>a\<^bold>p H \<brangle> "
+lemma sel_\<nu>app: " \<^bold>p\<^bold>r\<^bold>o\<^bold>c op_sel \<blangle> R\<heavy_comma> a \<tycolon> T\<heavy_comma> b \<tycolon> T\<heavy_comma> c \<tycolon> \<bool>\<heavy_comma> \<^bold>h\<^bold>e\<^bold>a\<^bold>p Nothing \<longmapsto> R\<heavy_comma> (if c then a else b) \<tycolon> T\<heavy_comma> \<^bold>h\<^bold>e\<^bold>a\<^bold>p Nothing \<brangle> "
   unfolding Procedure_def op_sel_def by (auto simp add: nu_exps)
 
 subsubsection \<open>if\<close>
@@ -245,32 +246,36 @@ subsubsection \<open>constant\<close>
 
 definition op_const_int :: "('w::len) itself \<Rightarrow> ('w::len) word \<Rightarrow> ('r::stack) \<longmapsto> 'w word \<times> 'r"
   where "op_const_int _ c = (\<lambda>(heap,r). Success (heap,c,r))"
-theorem const_nat_\<nu>app: "\<^bold>p\<^bold>r\<^bold>o\<^bold>c op_const_int TYPE('w::len) c \<blangle> R\<heavy_comma> \<^bold>h\<^bold>e\<^bold>a\<^bold>p H \<longmapsto> R \<heavy_comma> unat c \<tycolon> \<nat>['w]\<heavy_comma> \<^bold>h\<^bold>e\<^bold>a\<^bold>p H \<brangle>"
+theorem const_nat_\<nu>app: "\<^bold>p\<^bold>r\<^bold>o\<^bold>c op_const_int TYPE('w::len) c \<blangle> R\<heavy_comma> \<^bold>h\<^bold>e\<^bold>a\<^bold>p Nothing \<longmapsto> R \<heavy_comma> unat c \<tycolon> \<nat>['w]\<heavy_comma> \<^bold>h\<^bold>e\<^bold>a\<^bold>p Nothing \<brangle>"
   unfolding \<nu>def op_const_int_def by (auto simp add: nu_exps)
 (* theorem const_nat_round_\<nu>app: "\<^bold>p\<^bold>r\<^bold>o\<^bold>c op_const_int TYPE('w::len) (of_nat n) \<blangle> R \<longmapsto> R \<heavy_comma> n \<tycolon> \<nat>\<^sup>r['w] \<brangle>"
   unfolding \<nu>def op_const_int_def by auto *)
 
 lemma [\<nu>intro]:
   "\<^bold>p\<^bold>r\<^bold>e\<^bold>m\<^bold>i\<^bold>s\<^bold>e (numeral x :: nat) < 2^LENGTH('w) \<Longrightarrow>
-   \<^bold>c\<^bold>o\<^bold>n\<^bold>s\<^bold>t\<^bold>r\<^bold>u\<^bold>c\<^bold>t ((numeral x) \<tycolon> \<nat>['w]) \<^bold>b\<^bold>y \<^bold>p\<^bold>r\<^bold>o\<^bold>c op_const_int TYPE('w::len) (Word.of_nat (numeral x)) \<blangle> R\<heavy_comma> \<^bold>h\<^bold>e\<^bold>a\<^bold>p H \<longmapsto> R \<heavy_comma> (numeral x) \<tycolon> \<nat>['w]\<heavy_comma> \<^bold>h\<^bold>e\<^bold>a\<^bold>p H \<brangle>"
+   \<^bold>c\<^bold>o\<^bold>n\<^bold>s\<^bold>t\<^bold>r\<^bold>u\<^bold>c\<^bold>t ((numeral x) \<tycolon> \<nat>['w]) \<^bold>b\<^bold>y \<^bold>p\<^bold>r\<^bold>o\<^bold>c op_const_int TYPE('w::len) (Word.of_nat (numeral x))
+    \<blangle> R\<heavy_comma> \<^bold>h\<^bold>e\<^bold>a\<^bold>p Nothing \<longmapsto> R \<heavy_comma> (numeral x) \<tycolon> \<nat>['w]\<heavy_comma> \<^bold>h\<^bold>e\<^bold>a\<^bold>p Nothing \<brangle>"
   unfolding op_const_int_def \<nu>def including show_more1 by (auto simp add: nu_exps) (metis mod_if unat_bintrunc unat_numeral)
   \<comment> \<open>Only literal number could be constructed automatically\<close>
 lemma [\<nu>intro]:
-  "\<^bold>c\<^bold>o\<^bold>n\<^bold>s\<^bold>t\<^bold>r\<^bold>u\<^bold>c\<^bold>t (0 \<tycolon> \<nat>['w]) \<^bold>b\<^bold>y \<^bold>p\<^bold>r\<^bold>o\<^bold>c op_const_int TYPE('w::len) 0 \<blangle> R\<heavy_comma> \<^bold>h\<^bold>e\<^bold>a\<^bold>p H \<longmapsto> R \<heavy_comma> 0 \<tycolon> \<nat>['w]\<heavy_comma> \<^bold>h\<^bold>e\<^bold>a\<^bold>p H \<brangle>"
+  "\<^bold>c\<^bold>o\<^bold>n\<^bold>s\<^bold>t\<^bold>r\<^bold>u\<^bold>c\<^bold>t (0 \<tycolon> \<nat>['w]) \<^bold>b\<^bold>y \<^bold>p\<^bold>r\<^bold>o\<^bold>c op_const_int TYPE('w::len) 0
+    \<blangle> R\<heavy_comma> \<^bold>h\<^bold>e\<^bold>a\<^bold>p Nothing \<longmapsto> R \<heavy_comma> 0 \<tycolon> \<nat>['w]\<heavy_comma> \<^bold>h\<^bold>e\<^bold>a\<^bold>p Nothing \<brangle>"
   unfolding AutoConstruct_def using const_nat_\<nu>app by (metis unat_0) 
 lemma [\<nu>intro]:
-  "\<^bold>c\<^bold>o\<^bold>n\<^bold>s\<^bold>t\<^bold>r\<^bold>u\<^bold>c\<^bold>t (1 \<tycolon> \<nat>['w]) \<^bold>b\<^bold>y \<^bold>p\<^bold>r\<^bold>o\<^bold>c op_const_int TYPE('w::len) 1 \<blangle> R\<heavy_comma> \<^bold>h\<^bold>e\<^bold>a\<^bold>p H \<longmapsto> R\<heavy_comma> 1 \<tycolon> \<nat>['w]\<heavy_comma> \<^bold>h\<^bold>e\<^bold>a\<^bold>p H \<brangle>"
+  "\<^bold>c\<^bold>o\<^bold>n\<^bold>s\<^bold>t\<^bold>r\<^bold>u\<^bold>c\<^bold>t (1 \<tycolon> \<nat>['w]) \<^bold>b\<^bold>y \<^bold>p\<^bold>r\<^bold>o\<^bold>c op_const_int TYPE('w::len) 1
+    \<blangle> R\<heavy_comma> \<^bold>h\<^bold>e\<^bold>a\<^bold>p Nothing \<longmapsto> R\<heavy_comma> 1 \<tycolon> \<nat>['w]\<heavy_comma> \<^bold>h\<^bold>e\<^bold>a\<^bold>p Nothing \<brangle>"
   unfolding AutoConstruct_def using const_nat_\<nu>app by (metis unat_1)
 
 lemma [\<nu>intro]:
   "\<^bold>p\<^bold>r\<^bold>e\<^bold>m\<^bold>i\<^bold>s\<^bold>e (numeral x :: nat) < 2^LENGTH('w) \<Longrightarrow>
-   \<^bold>c\<^bold>o\<^bold>n\<^bold>s\<^bold>t\<^bold>r\<^bold>u\<^bold>c\<^bold>t ((numeral x) \<tycolon> \<nat>\<^sup>r['w]) \<^bold>b\<^bold>y \<^bold>p\<^bold>r\<^bold>o\<^bold>c op_const_int TYPE('w::len) (Word.of_nat (numeral x)) \<blangle> R\<heavy_comma> \<^bold>h\<^bold>e\<^bold>a\<^bold>p H \<longmapsto> R\<heavy_comma> (numeral x) \<tycolon> \<nat>\<^sup>r['w]\<heavy_comma> \<^bold>h\<^bold>e\<^bold>a\<^bold>p H \<brangle>"
+   \<^bold>c\<^bold>o\<^bold>n\<^bold>s\<^bold>t\<^bold>r\<^bold>u\<^bold>c\<^bold>t ((numeral x) \<tycolon> \<nat>\<^sup>r['w]) \<^bold>b\<^bold>y \<^bold>p\<^bold>r\<^bold>o\<^bold>c op_const_int TYPE('w::len) (Word.of_nat (numeral x))
+    \<blangle> R\<heavy_comma> \<^bold>h\<^bold>e\<^bold>a\<^bold>p Nothing \<longmapsto> R\<heavy_comma> (numeral x) \<tycolon> \<nat>\<^sup>r['w]\<heavy_comma> \<^bold>h\<^bold>e\<^bold>a\<^bold>p Nothing \<brangle>"
   unfolding op_const_int_def \<nu>def including show_more1 by (auto simp add: nu_exps)
 lemma [\<nu>intro]:
-  "\<^bold>c\<^bold>o\<^bold>n\<^bold>s\<^bold>t\<^bold>r\<^bold>u\<^bold>c\<^bold>t (0 \<tycolon> \<nat>\<^sup>r['w]) \<^bold>b\<^bold>y \<^bold>p\<^bold>r\<^bold>o\<^bold>c op_const_int TYPE('w::len) 0 \<blangle> R\<heavy_comma> \<^bold>h\<^bold>e\<^bold>a\<^bold>p H \<longmapsto> R\<heavy_comma> 0 \<tycolon> \<nat>\<^sup>r['w]\<heavy_comma> \<^bold>h\<^bold>e\<^bold>a\<^bold>p H \<brangle>"
+  "\<^bold>c\<^bold>o\<^bold>n\<^bold>s\<^bold>t\<^bold>r\<^bold>u\<^bold>c\<^bold>t (0 \<tycolon> \<nat>\<^sup>r['w]) \<^bold>b\<^bold>y \<^bold>p\<^bold>r\<^bold>o\<^bold>c op_const_int TYPE('w::len) 0 \<blangle> R\<heavy_comma> \<^bold>h\<^bold>e\<^bold>a\<^bold>p Nothing \<longmapsto> R\<heavy_comma> 0 \<tycolon> \<nat>\<^sup>r['w]\<heavy_comma> \<^bold>h\<^bold>e\<^bold>a\<^bold>p Nothing \<brangle>"
   unfolding op_const_int_def \<nu>def including show_more1 by (auto simp add: nu_exps)
 lemma [\<nu>intro]:
-  "\<^bold>c\<^bold>o\<^bold>n\<^bold>s\<^bold>t\<^bold>r\<^bold>u\<^bold>c\<^bold>t (1 \<tycolon> \<nat>\<^sup>r['w]) \<^bold>b\<^bold>y \<^bold>p\<^bold>r\<^bold>o\<^bold>c op_const_int TYPE('w::len) 1 \<blangle> R\<heavy_comma> \<^bold>h\<^bold>e\<^bold>a\<^bold>p H \<longmapsto> R\<heavy_comma> 1 \<tycolon> \<nat>\<^sup>r['w]\<heavy_comma> \<^bold>h\<^bold>e\<^bold>a\<^bold>p H \<brangle>"
+  "\<^bold>c\<^bold>o\<^bold>n\<^bold>s\<^bold>t\<^bold>r\<^bold>u\<^bold>c\<^bold>t (1 \<tycolon> \<nat>\<^sup>r['w]) \<^bold>b\<^bold>y \<^bold>p\<^bold>r\<^bold>o\<^bold>c op_const_int TYPE('w::len) 1 \<blangle> R\<heavy_comma> \<^bold>h\<^bold>e\<^bold>a\<^bold>p Nothing \<longmapsto> R\<heavy_comma> 1 \<tycolon> \<nat>\<^sup>r['w]\<heavy_comma> \<^bold>h\<^bold>e\<^bold>a\<^bold>p Nothing \<brangle>"
   unfolding op_const_int_def \<nu>def including show_more1 by (auto simp add: nu_exps)
 
 (* schematic_goal "\<^bold>c\<^bold>o\<^bold>n\<^bold>s\<^bold>t\<^bold>r\<^bold>u\<^bold>c\<^bold>t 3 \<^bold>b\<^bold>y \<^bold>p\<^bold>r\<^bold>o\<^bold>c ?f
@@ -290,10 +295,12 @@ definition op_add :: "'a itself \<Rightarrow> ('a::len) word \<times> ('a::len) 
 declare op_add_def[\<nu>instr]
 
 theorem add_nat_\<nu>app[\<nu>overload +]:
-  "\<^bold>p\<^bold>r\<^bold>e\<^bold>m\<^bold>i\<^bold>s\<^bold>e x + y < 2^LENGTH('b::len) \<longrightarrow> \<^bold>p\<^bold>r\<^bold>o\<^bold>c op_add TYPE('b) \<blangle> R\<heavy_comma> x \<tycolon> \<nat>['b] \<heavy_comma> y \<tycolon> \<nat>['b]\<heavy_comma> \<^bold>h\<^bold>e\<^bold>a\<^bold>p H \<longmapsto> R\<heavy_comma> x + y \<tycolon> \<nat>['b]\<heavy_comma> \<^bold>h\<^bold>e\<^bold>a\<^bold>p H \<brangle>"
+  "\<^bold>p\<^bold>r\<^bold>e\<^bold>m\<^bold>i\<^bold>s\<^bold>e x + y < 2^LENGTH('b::len) \<longrightarrow>
+    \<^bold>p\<^bold>r\<^bold>o\<^bold>c op_add TYPE('b) \<blangle> R\<heavy_comma> x \<tycolon> \<nat>['b] \<heavy_comma> y \<tycolon> \<nat>['b]\<heavy_comma> \<^bold>h\<^bold>e\<^bold>a\<^bold>p Nothing \<longmapsto> R\<heavy_comma> x + y \<tycolon> \<nat>['b]\<heavy_comma> \<^bold>h\<^bold>e\<^bold>a\<^bold>p Nothing \<brangle>"
   unfolding op_add_def Procedure_def by (auto simp add: of_nat_inverse nu_exps)
 
-theorem add_nat_round[\<nu>overload +]: "\<^bold>p\<^bold>r\<^bold>o\<^bold>c op_add TYPE('b) \<blangle> R\<heavy_comma> x \<tycolon> \<nat>\<^sup>r['b::len]\<heavy_comma> y \<tycolon> \<nat>\<^sup>r['b]\<heavy_comma> \<^bold>h\<^bold>e\<^bold>a\<^bold>p H \<longmapsto> R\<heavy_comma> (x + y) \<tycolon> \<nat>\<^sup>r['b]\<heavy_comma> \<^bold>h\<^bold>e\<^bold>a\<^bold>p H \<brangle>"
+theorem add_nat_round[\<nu>overload +]:
+  "\<^bold>p\<^bold>r\<^bold>o\<^bold>c op_add TYPE('b) \<blangle> R\<heavy_comma> x \<tycolon> \<nat>\<^sup>r['b::len]\<heavy_comma> y \<tycolon> \<nat>\<^sup>r['b]\<heavy_comma> \<^bold>h\<^bold>e\<^bold>a\<^bold>p Nothing \<longmapsto> R\<heavy_comma> (x + y) \<tycolon> \<nat>\<^sup>r['b]\<heavy_comma> \<^bold>h\<^bold>e\<^bold>a\<^bold>p Nothing \<brangle>"
   unfolding op_add_def Procedure_def by (auto simp add: nu_exps)
 
 (* theorem add_nat_mod[\<nu>overload round_add]:
@@ -306,7 +313,8 @@ definition op_sub :: "('a::len) itself \<Rightarrow> 'a word \<times> 'a word \<
   where "op_sub _ = (\<lambda>(h,a,b,r) \<Rightarrow> Success (h,b - a, r))"
 declare op_sub_def[\<nu>instr]
 theorem sub_nat_\<nu>app[\<nu>overload -]:
-    "\<^bold>p\<^bold>r\<^bold>e\<^bold>m\<^bold>i\<^bold>s\<^bold>e y \<le> x \<longrightarrow> \<^bold>p\<^bold>r\<^bold>o\<^bold>c op_sub TYPE('w::len) \<blangle> R\<heavy_comma> x \<tycolon> \<nat>['w] \<heavy_comma> y \<tycolon> \<nat>['w]\<heavy_comma> \<^bold>h\<^bold>e\<^bold>a\<^bold>p H \<longmapsto> R\<heavy_comma> x - y \<tycolon> \<nat>['w]\<heavy_comma> \<^bold>h\<^bold>e\<^bold>a\<^bold>p H \<brangle>"
+    "\<^bold>p\<^bold>r\<^bold>e\<^bold>m\<^bold>i\<^bold>s\<^bold>e y \<le> x \<longrightarrow>
+    \<^bold>p\<^bold>r\<^bold>o\<^bold>c op_sub TYPE('w::len) \<blangle> R\<heavy_comma> x \<tycolon> \<nat>['w] \<heavy_comma> y \<tycolon> \<nat>['w]\<heavy_comma> \<^bold>h\<^bold>e\<^bold>a\<^bold>p Nothing \<longmapsto> R\<heavy_comma> x - y \<tycolon> \<nat>['w]\<heavy_comma> \<^bold>h\<^bold>e\<^bold>a\<^bold>p Nothing \<brangle>"
   unfolding \<nu>def op_sub_def by (auto simp add: nu_exps) (meson unat_sub_if_size)
   
 subsubsection \<open>less\<close>
@@ -315,13 +323,13 @@ definition op_lt :: " ('w::len) itself \<Rightarrow> 'w word \<times> 'w word \<
   where "op_lt _ = (\<lambda>(h,a,b,r).  Success (h, (if  b < a then 1 else 0), r))"
 declare op_lt_def[\<nu>instr]
 theorem op_lt_\<nu>app[\<nu>overload <]:
-    "\<^bold>p\<^bold>r\<^bold>o\<^bold>c op_lt TYPE('w::len) \<blangle> R\<heavy_comma> x \<tycolon> \<nat>['w]\<heavy_comma> y \<tycolon> \<nat>['w]\<heavy_comma> \<^bold>h\<^bold>e\<^bold>a\<^bold>p H \<longmapsto> R\<heavy_comma> (x < y) \<tycolon> \<bool>\<heavy_comma> \<^bold>h\<^bold>e\<^bold>a\<^bold>p H \<brangle>"
+    "\<^bold>p\<^bold>r\<^bold>o\<^bold>c op_lt TYPE('w::len) \<blangle> R\<heavy_comma> x \<tycolon> \<nat>['w]\<heavy_comma> y \<tycolon> \<nat>['w]\<heavy_comma> \<^bold>h\<^bold>e\<^bold>a\<^bold>p Nothing \<longmapsto> R\<heavy_comma> (x < y) \<tycolon> \<bool>\<heavy_comma> \<^bold>h\<^bold>e\<^bold>a\<^bold>p Nothing \<brangle>"
   unfolding \<nu>def op_lt_def by (auto simp add: word_less_nat_alt nu_exps)
 
 definition op_le :: " ('w::len) itself \<Rightarrow> 'w word \<times> 'w word \<times> ('r::lrep) \<longmapsto> 1 word \<times> 'r "
   where "op_le _ = (\<lambda>(h,a,b,r).  Success (h, (if  b \<le> a then 1 else 0), r))"
 theorem op_le_\<nu>app[\<nu>overload \<le>]:
-    "\<^bold>p\<^bold>r\<^bold>o\<^bold>c op_le TYPE('w::len) \<blangle> R\<heavy_comma> x \<tycolon> \<nat>['w]\<heavy_comma> y \<tycolon> \<nat>['w]\<heavy_comma> \<^bold>h\<^bold>e\<^bold>a\<^bold>p H \<longmapsto> R\<heavy_comma> (x \<le> y) \<tycolon> \<bool>\<heavy_comma> \<^bold>h\<^bold>e\<^bold>a\<^bold>p H \<brangle>"
+    "\<^bold>p\<^bold>r\<^bold>o\<^bold>c op_le TYPE('w::len) \<blangle> R\<heavy_comma> x \<tycolon> \<nat>['w]\<heavy_comma> y \<tycolon> \<nat>['w]\<heavy_comma> \<^bold>h\<^bold>e\<^bold>a\<^bold>p Nothing \<longmapsto> R\<heavy_comma> (x \<le> y) \<tycolon> \<bool>\<heavy_comma> \<^bold>h\<^bold>e\<^bold>a\<^bold>p Nothing \<brangle>"
   unfolding \<nu>def op_le_def by (auto simp add: word_le_nat_alt nu_exps)
 
 subsubsection \<open>bit-wise not\<close>
@@ -329,7 +337,8 @@ subsubsection \<open>bit-wise not\<close>
 definition op_not :: "('w::len) itself \<Rightarrow> 'w word \<times> ('r::stack) \<longmapsto> 'w word \<times> 'r"
   where "op_not len = (\<lambda>(h,x,r). Success (h,not x,r))"
 
-lemma boolean_not_\<nu>app[\<nu>overload not]: "\<^bold>p\<^bold>r\<^bold>o\<^bold>c op_not TYPE(1) \<blangle> R\<heavy_comma> x \<tycolon> \<bool>\<heavy_comma> \<^bold>h\<^bold>e\<^bold>a\<^bold>p H \<longmapsto> R\<heavy_comma> \<not> x \<tycolon> \<bool>\<heavy_comma> \<^bold>h\<^bold>e\<^bold>a\<^bold>p H \<brangle>"
+lemma boolean_not_\<nu>app[\<nu>overload not]:
+    "\<^bold>p\<^bold>r\<^bold>o\<^bold>c op_not TYPE(1) \<blangle> R\<heavy_comma> x \<tycolon> \<bool>\<heavy_comma> \<^bold>h\<^bold>e\<^bold>a\<^bold>p Nothing \<longmapsto> R\<heavy_comma> \<not> x \<tycolon> \<bool>\<heavy_comma> \<^bold>h\<^bold>e\<^bold>a\<^bold>p Nothing \<brangle>"
   unfolding Procedure_def op_not_def apply (auto simp add: lrep_exps nu_exps)
   by (metis even_take_bit_eq even_zero iszero_def odd_numeral one_neq_zero)
 
@@ -338,7 +347,7 @@ subsubsection \<open>equal\<close>
 definition op_equal :: " ('a::{ceq,lrep}) \<times> 'a \<times> ('r::stack) \<longmapsto> 1 word \<times> 'r"
   where "op_equal = (\<lambda>(h,a,b,r). if ceqable h b a then Success (h,(if ceq b a then 1 else 0), r) else Fail)"
 theorem op_equal[\<nu>overload =]:
-  "\<nu>Equal N P eq \<longrightarrow> \<^bold>p\<^bold>r\<^bold>e\<^bold>m\<^bold>i\<^bold>s\<^bold>e P a b \<longrightarrow> \<^bold>p\<^bold>r\<^bold>o\<^bold>c op_equal \<blangle> R\<heavy_comma> a \<tycolon> N\<heavy_comma> b \<tycolon> N\<heavy_comma> \<^bold>h\<^bold>e\<^bold>a\<^bold>p H \<longmapsto> R\<heavy_comma> eq a b \<tycolon> \<bool>\<heavy_comma> \<^bold>h\<^bold>e\<^bold>a\<^bold>p H \<brangle>"
+  "\<nu>Equal N P eq \<longrightarrow> \<^bold>p\<^bold>r\<^bold>e\<^bold>m\<^bold>i\<^bold>s\<^bold>e P a b \<longrightarrow> \<^bold>p\<^bold>r\<^bold>o\<^bold>c op_equal \<blangle> R\<heavy_comma> a \<tycolon> N\<heavy_comma> b \<tycolon> N\<heavy_comma> \<^bold>h\<^bold>e\<^bold>a\<^bold>p Nothing \<longmapsto> R\<heavy_comma> eq a b \<tycolon> \<bool>\<heavy_comma> \<^bold>h\<^bold>e\<^bold>a\<^bold>p Nothing \<brangle>"
   unfolding \<nu>def op_equal_def by (auto 0 6 simp add: nu_exps)
 
 section \<open>Tuple Operations\<close>
@@ -350,7 +359,8 @@ subsubsection \<open>op_constr_tuple\<close>
 definition op_constr_tuple :: "('a::field_list) \<times> ('r::stack) \<longmapsto> 'a tuple \<times> 'r"
   where "op_constr_tuple = (\<lambda>(h,a,r). Success (h, Tuple a, r))"
 
-theorem tup_\<nu>app: "\<^bold>p\<^bold>r\<^bold>o\<^bold>c op_constr_tuple \<blangle> R \<heavy_comma> x \<tycolon> X\<heavy_comma> \<^bold>h\<^bold>e\<^bold>a\<^bold>p H \<longmapsto> R \<heavy_comma> x \<tycolon> \<lbrace> X \<rbrace> \<heavy_comma> \<^bold>h\<^bold>e\<^bold>a\<^bold>p H \<brangle>"
+theorem tup_\<nu>app:
+    "\<^bold>p\<^bold>r\<^bold>o\<^bold>c op_constr_tuple \<blangle> R \<heavy_comma> x \<tycolon> X\<heavy_comma> \<^bold>h\<^bold>e\<^bold>a\<^bold>p Nothing \<longmapsto> R \<heavy_comma> x \<tycolon> \<lbrace> X \<rbrace> \<heavy_comma> \<^bold>h\<^bold>e\<^bold>a\<^bold>p Nothing \<brangle>"
   unfolding op_constr_tuple_def Procedure_def by (simp add: pair_forall nu_exps)
 
 subsubsection \<open>op_destr_tuple\<close>
@@ -358,7 +368,8 @@ subsubsection \<open>op_destr_tuple\<close>
 definition op_destr_tuple :: "('a::field_list) tuple \<times> ('r::stack) \<longmapsto> 'a \<times> 'r"
   where "op_destr_tuple s = (case s of (h,Tuple a, r) \<Rightarrow> Success (h,a,r))"
 
-theorem det_\<nu>app: "\<^bold>p\<^bold>r\<^bold>o\<^bold>c op_destr_tuple \<blangle> R\<heavy_comma> x \<tycolon> \<lbrace> X \<rbrace>\<heavy_comma> \<^bold>h\<^bold>e\<^bold>a\<^bold>p H \<longmapsto> R\<heavy_comma> x \<tycolon> X\<heavy_comma> \<^bold>h\<^bold>e\<^bold>a\<^bold>p H \<brangle>"
+theorem det_\<nu>app:
+    "\<^bold>p\<^bold>r\<^bold>o\<^bold>c op_destr_tuple \<blangle> R\<heavy_comma> x \<tycolon> \<lbrace> X \<rbrace>\<heavy_comma> \<^bold>h\<^bold>e\<^bold>a\<^bold>p Nothing \<longmapsto> R\<heavy_comma> x \<tycolon> X\<heavy_comma> \<^bold>h\<^bold>e\<^bold>a\<^bold>p Nothing \<brangle>"
   unfolding Procedure_def op_destr_tuple_def by (simp add: tuple_forall pair_forall nu_exps)
 
 subsection \<open>Field Index\<close>
@@ -411,20 +422,20 @@ definition op_shift_pointer :: "llty \<Rightarrow> size_t word \<times> memptr \
   
 theorem op_shift_pointer[\<nu>overload +]:
   "\<^bold>p\<^bold>r\<^bold>e\<^bold>m\<^bold>i\<^bold>s\<^bold>e address_llty addr = ty \<Longrightarrow> \<^bold>p\<^bold>r\<^bold>e\<^bold>m\<^bold>i\<^bold>s\<^bold>e offset_of addr + delta \<le> address_len addr \<Longrightarrow>
-  \<^bold>p\<^bold>r\<^bold>o\<^bold>c op_shift_pointer ty \<blangle> R\<heavy_comma> addr \<tycolon> Pointer\<heavy_comma> delta \<tycolon> \<nat>[size_t]\<heavy_comma> \<^bold>h\<^bold>e\<^bold>a\<^bold>p H \<longmapsto>
-      R\<heavy_comma> addr ||+ delta \<tycolon> Pointer\<heavy_comma> \<^bold>h\<^bold>e\<^bold>a\<^bold>p H \<brangle>"
+  \<^bold>p\<^bold>r\<^bold>o\<^bold>c op_shift_pointer ty \<blangle> R\<heavy_comma> addr \<tycolon> Pointer\<heavy_comma> delta \<tycolon> \<nat>[size_t]\<heavy_comma> \<^bold>h\<^bold>e\<^bold>a\<^bold>p Nothing \<longmapsto>
+      R\<heavy_comma> addr ||+ delta \<tycolon> Pointer\<heavy_comma> \<^bold>h\<^bold>e\<^bold>a\<^bold>p Nothing \<brangle>"
   unfolding \<nu>def op_shift_pointer_def by (cases addr) (auto simp add: lrep_exps same_addr_offset_def nu_exps)
 
 
 theorem op_shift_pointer_slice[ unfolded Separation_assoc, \<nu>overload split ]:
   "\<^bold>p\<^bold>r\<^bold>e\<^bold>m\<^bold>i\<^bold>s\<^bold>e n < length xs \<longrightarrow>
-  \<^bold>p\<^bold>r\<^bold>o\<^bold>c op_shift_pointer LLTY('p) \<blangle> R\<heavy_comma> addr \<tycolon> Pointer\<heavy_comma> n \<tycolon> \<nat>[size_t]\<heavy_comma> \<^bold>h\<^bold>e\<^bold>a\<^bold>p H \<heavy_asterisk> addr \<R_arr_tail> xs \<tycolon> Array T
-      \<longmapsto> R\<heavy_comma> addr ||+ n \<tycolon> Pointer\<heavy_comma> \<^bold>h\<^bold>e\<^bold>a\<^bold>p H \<heavy_asterisk> (addr \<R_arr_tail> take n xs \<tycolon> Array T \<heavy_asterisk> shift_addr addr n \<R_arr_tail> drop n xs \<tycolon> Array T) \<brangle>"
+  \<^bold>p\<^bold>r\<^bold>o\<^bold>c op_shift_pointer LLTY('p) \<blangle> R\<heavy_comma> addr \<tycolon> Pointer\<heavy_comma> n \<tycolon> \<nat>[size_t]\<heavy_comma> \<^bold>h\<^bold>e\<^bold>a\<^bold>p addr \<R_arr_tail> xs \<tycolon> Array T
+      \<longmapsto> R\<heavy_comma> addr ||+ n \<tycolon> Pointer\<heavy_comma> \<^bold>h\<^bold>e\<^bold>a\<^bold>p (addr \<R_arr_tail> take n xs \<tycolon> Array T \<heavy_asterisk> shift_addr addr n \<R_arr_tail> drop n xs \<tycolon> Array T) \<brangle>"
   for T :: "('p::field, 'x) \<nu>"
   unfolding \<nu>def op_shift_pointer_def Array_def Heap_Divider_def apply (cases addr)
   apply (auto simp add: lrep_exps same_addr_offset_def raw_offset_of_def distrib_right nu_exps
         add.commute add.left_commute intro: heap_split_id)
-  subgoal for x1 x2 aa h1 h2 b
+  subgoal for x1 x2 aa b H h1 h2
     by (rule heap_split_id, simp, rule heap_split_by_addr_set[of _ _ "{(x1 |+ x2 + i) | i. i < n}"]) (auto simp add: nu_exps)
   done
 
@@ -478,15 +489,16 @@ definition op_alloc :: "('x::{zero,field}) itself \<Rightarrow> size_t word \<ti
       
 theorem alloc_array_\<nu>app:
   "\<^bold>p\<^bold>a\<^bold>r\<^bold>a\<^bold>m N \<Longrightarrow> \<nu>Zero N zero \<Longrightarrow> \<^bold>p\<^bold>r\<^bold>o\<^bold>c op_alloc TYPE('x)
-      \<blangle> R\<heavy_comma> n \<tycolon> \<nat>[size_t] \<heavy_comma> \<^bold>h\<^bold>e\<^bold>a\<^bold>p H
-        \<longmapsto> (\<exists>*seg. (R\<heavy_comma> (seg |+ 0) \<tycolon> Pointer \<heavy_comma> \<^bold>h\<^bold>e\<^bold>a\<^bold>p H \<heavy_asterisk> (seg |+ 0) \<R_arr_tail> replicate n zero \<tycolon> Array N)) \<brangle>"
+      \<blangle> R\<heavy_comma> n \<tycolon> \<nat>[size_t] \<heavy_comma> \<^bold>h\<^bold>e\<^bold>a\<^bold>p Nothing
+        \<longmapsto> (\<exists>*seg. (R\<heavy_comma> (seg |+ 0) \<tycolon> Pointer \<heavy_comma> \<^bold>h\<^bold>e\<^bold>a\<^bold>p (seg |+ 0) \<R_arr_tail> replicate n zero \<tycolon> Array N)) \<brangle>"
   for N :: "('x::{zero,field},'b)\<nu>"
   unfolding \<nu>def op_alloc_def Array_def Heap_Divider_def
   apply (auto simp add: lrep_exps list_all2_conv_all_nth Let_def same_addr_offset_def nu_exps)
   apply (rule malloc_split, simp add: heap_assignN_eval)
   apply (auto simp add: heap_assignN_eval nu_exps) done
 
-proc alloc : \<open>R\<heavy_comma> \<^bold>h\<^bold>e\<^bold>a\<^bold>p H\<close> \<longmapsto> \<open>\<exists>*ptr. (R\<heavy_comma> ptr \<tycolon> Pointer\<heavy_comma> \<^bold>h\<^bold>e\<^bold>a\<^bold>p H \<heavy_asterisk> ptr \<R_arr_tail> zero \<tycolon> Ref T)\<close>
+
+proc alloc : \<open>R\<heavy_comma> \<^bold>h\<^bold>e\<^bold>a\<^bold>p Nothing\<close> \<longmapsto> \<open>\<exists>*ptr. (R\<heavy_comma> ptr \<tycolon> Pointer\<heavy_comma> \<^bold>h\<^bold>e\<^bold>a\<^bold>p ptr \<R_arr_tail> zero \<tycolon> Ref T)\<close>
   requires "\<^bold>p\<^bold>a\<^bold>r\<^bold>a\<^bold>m T" and [\<nu>intro]: "\<nu>Zero T zero"
   have A[simp]: "replicate 1 zero = [zero]" by (simp add: One_nat_def)
   \<bullet>\<open>1 \<tycolon> \<nat>[size_t]\<close> alloc_array T
@@ -519,7 +531,7 @@ proc i_load_n[\<nu>overload "\<up>:"]:
   \<open>a \<tycolon> Pointer\<heavy_comma> i \<tycolon> \<nat>[size_t]\<heavy_comma> \<^bold>h\<^bold>e\<^bold>a\<^bold>p H \<heavy_asterisk> a \<R_arr_tail> xs \<tycolon> Array X\<close> \<longmapsto> \<open>gt (xs ! i) \<tycolon> Y\<heavy_comma> \<^bold>h\<^bold>e\<^bold>a\<^bold>p H \<heavy_asterisk> a \<R_arr_tail> xs \<tycolon> Array X\<close>
   for Y :: "('y::field, 'd) \<nu>"
   requires [used]: "\<^bold>p\<^bold>r\<^bold>e\<^bold>m\<^bold>i\<^bold>s\<^bold>e i < length xs" and idx: "FieldIndex field_index Y X gt mp"
-  \<bullet> + \<up>: idx
+  \<bullet> +\<up>: idx
   finish
 
 lemmas [ \<nu>overload "\<up>" ] = i_load_n_\<nu>app[THEN mp, THEN mp, OF _ FieldIndex_here, unfolded atomize_imp, simplified]
@@ -537,12 +549,12 @@ definition op_store :: " llty \<Rightarrow> ('a::lrep,'a,'ax,'ax) index \<Righta
 theorem op_store[ \<nu>overload "\<down>:" ]:
   "FieldIndex field_index Y X gt mp \<longrightarrow>
   \<^bold>p\<^bold>r\<^bold>o\<^bold>c op_store LLTY('x) field_index
-    \<blangle> R\<heavy_comma> addr \<tycolon> Pointer\<heavy_comma> y \<tycolon> Y\<heavy_comma> \<^bold>h\<^bold>e\<^bold>a\<^bold>p H \<heavy_asterisk> addr \<R_arr_tail> x \<tycolon> Ref X \<longmapsto> R \<heavy_comma> addr \<tycolon> Pointer \<heavy_comma> \<^bold>h\<^bold>e\<^bold>a\<^bold>p H \<heavy_asterisk> addr \<R_arr_tail> mp (\<lambda>_. y) x \<tycolon> Ref X\<brangle> "
+    \<blangle> R\<heavy_comma> addr \<tycolon> Pointer\<heavy_comma> y \<tycolon> Y\<heavy_comma> \<^bold>h\<^bold>e\<^bold>a\<^bold>p addr \<R_arr_tail> x \<tycolon> Ref X \<longmapsto> R \<heavy_comma> addr \<tycolon> Pointer \<heavy_comma> \<^bold>h\<^bold>e\<^bold>a\<^bold>p addr \<R_arr_tail> mp (\<lambda>_. y) x \<tycolon> Ref X\<brangle> "
   for X :: "('x::field, 'c) \<nu>"
   unfolding op_store_def Procedure_def FieldIndex_def \<nu>index_def Heap_Divider_def Stack_Delimiter_def
   apply (cases field_index, cases addr)
   apply (auto simp add: lrep_exps Let_def nu_exps split: option.split iff: addr_allocated_def)
-  subgoal premises prems for x1 x2 x1a x2a aa ofs b x2b h1 h2 proof -
+  subgoal premises prems for x1 x2 x1a x2a aa ofs b x2b H h1 h2 proof -
     have t1: "\<And>v. (h1 ++ h2)(MemAddress (x1a |+ x2a) \<mapsto> v) = h1 ++ (h2(MemAddress (x1a |+ x2a) \<mapsto> v))"
       using prems disjoint_rewR by simp
     have t2: "\<And>v.  dom (h2(MemAddress (x1a |+ x2a) \<mapsto> v)) = dom h2"
@@ -554,10 +566,12 @@ theorem op_store[ \<nu>overload "\<down>:" ]:
 lemmas [ \<nu>overload "\<down>" ] = op_store[THEN mp, OF FieldIndex_here, simplified]
 
 proc i_store_n[\<nu>overload "\<down>:"]:
-  \<open>R\<heavy_comma> a \<tycolon> Pointer\<heavy_comma> i \<tycolon> \<nat>[size_t]\<heavy_comma> y \<tycolon> Y \<heavy_comma> \<^bold>h\<^bold>e\<^bold>a\<^bold>p H \<heavy_asterisk> a \<R_arr_tail> xs \<tycolon> Array X\<close> \<longmapsto> \<open>R\<heavy_comma> \<^bold>h\<^bold>e\<^bold>a\<^bold>p H \<heavy_asterisk> a \<R_arr_tail> xs[i := mp (\<lambda>_. y) (xs ! i)] \<tycolon> Array X\<close>
+  \<open>R\<heavy_comma> a \<tycolon> Pointer\<heavy_comma> i \<tycolon> \<nat>[size_t]\<heavy_comma> y \<tycolon> Y \<heavy_comma> \<^bold>h\<^bold>e\<^bold>a\<^bold>p a \<R_arr_tail> xs \<tycolon> Array X\<close> \<longmapsto> \<open>R\<heavy_comma> \<^bold>h\<^bold>e\<^bold>a\<^bold>p a \<R_arr_tail> xs[i := mp (\<lambda>_. y) (xs ! i)] \<tycolon> Array X\<close>
   for Y :: "('y::field, 'd) \<nu>"
   requires [used]: "\<^bold>p\<^bold>r\<^bold>e\<^bold>m\<^bold>i\<^bold>s\<^bold>e i < length xs" and idx: "FieldIndex field_index Y X gt mp"
-  \<bullet> \<rightarrow> y + y \<down>: idx drop
+  \<bullet> \<rightarrow> y
+  \<bullet> + y
+  \<bullet> \<down>: idx drop
   finish
 
 lemmas [ \<nu>overload "\<down>" ] = i_store_n_\<nu>app[THEN mp, THEN mp, OF _ FieldIndex_here, unfolded atomize_imp, simplified]
